theories/logic/adequacy.v
@@ -42,7 +42,7 @@ Proof.
     iApply fupd_wp. iApply ("Hrel" $! (RefId 0 [])).
     iSplitR.
     + iExists _. by iFrame.
-    + rewrite tpool_mapsto_eq /tpool_mapsto_def.
+    + rewrite tpool_pointsto_eq /tpool_pointsto_def.
       by rewrite /to_tpool /= insert_empty map_fmap_singleton //.
   - iIntros (v).
     iDestruct 1 as (v') "[Hj Hinterp]".
@@ -50,7 +50,7 @@ Proof.
     iDestruct "Hinterp" as %Hinterp.
     iInv specN as (tp σ') ">[Hown Hsteps]" "Hclose"; iDestruct "Hsteps" as %Hsteps'.
     iDestruct "Hj" as "[#Hs Hj]".
-    rewrite tpool_mapsto_eq /tpool_mapsto_def /=.
+    rewrite tpool_pointsto_eq /tpool_pointsto_def /=.
     iCombine "Hown Hj" gives %Hvalid.
     move: Hvalid=> /auth_both_valid_discrete
        [/prod_included [/tpool_singleton_included Hv2 _] _].
